many new things

theories/InterpreterStrict.v
@@ -6,7 +6,7 @@ Require Int63.
 Import ListNotations.
 Open Scope string_scope.
 
-Require Import Malfunction.Malfunction Malfunction.Deserialize Ceres.Ceres.
+Require Import Malfunction.Malfunction.
 
 (* type value = *)
 (* | Block of int * value array *)
@@ -15,53 +15,16 @@ Require Import Malfunction.Malfunction Malfunction.Deserialize Ceres.Ceres.
 (* | Int of inttype * Z.t *)
 (* | Float of float *)
 (* | Thunk of value Lazy.t *)
-#[bypass_check(positivity)]
-Inductive break : Prop :=
-| B : (break -> break) -> break.
-
-Fixpoint prv (b : break) : False :=
-  match b with
-  | B f => prv (f (B f))
-  end.
-
-Goal False.
-Proof.
-  exact (prv (B (fun x => x))).
-Qed.
-
-#[bypass_check(positivity)]
-Inductive break_ : forall X : Prop, Prop :=
-| B_ (X : Prop) : (X -> break_ (break_ X)) -> break_ X.
-
-Fixpoint prv_ {X : Prop} (x : X) (b : break_ X) : False.
-Proof.
-  destruct b.
-  eapply prv_.
-  2: eapply H; eauto. 
-  econstructor. eauto.
-Qed.
-
-Goal ~ (forall P, P \/ ~ P).
-Proof.
-  intros lem.
-  unshelve eapply prv_. exact True. eauto.
-  destruct (lem (break_ True)) as [H | H].
-  - exact H.
-  - econstructor. econstructor. eauto.
-    intros h. destruct H. eauto.
-Qed.
 
 Inductive value :=
 | Block of int * array value      
 | Vec of vector_type * array value
-| Func of (value -> value)
+| Func of Ident.t * @Ident.Map.t value * t
 | value_Int of inttype * Z
 | Float of float
 | Thunk of value
 | fail of string
 .
-Scheme foo := Induction for value Sort Prop.
-Print foo.
 
 Definition add (x : string) (v : value) (locals : string -> value)  :=
   fun y =>
@@ -148,62 +111,9 @@ Definition comparison_eqb x1 x2 :=
   end.
 
 #[bypass_check(guard)]
-Fixpoint newlocals (interpret : @Ident.Map.t value -> t -> value) (recs : list (Ident.t * t)) locals (x : Ident.t) {struct x}:=
-  List.fold_right
-  (fun '(x,e) locals => Ident.Map.add x e locals)
-  (locals)
-  (List.map (fun '(x,e) =>
-    let v := match e with
-      | Mlambda _ => Func (fun arg => 
-         match interpret (fun x => newlocals interpret recs locals x) e with
-         | Func f => f arg
-         | _ => fail "bad recursive function binding"
-         end)
-      | _ => fail "recursive values must be functions"
-      end in
-    (x, v)) recs) x.
-
-Lemma newlocals_eqn (interpret : @Ident.Map.t value -> t -> value) recs locals (x : Ident.t) :
-  newlocals interpret recs locals x = 
-  List.fold_right
-  (fun '(x,e) locals => Ident.Map.add x e locals)
-  (locals)
-  (List.map (fun '(x,e) =>
-    let v := match e with
-      | Mlambda _ => Func (fun arg => 
-         match interpret (fun x => newlocals interpret recs locals x) e with
-         | Func f => f arg
-         | _ => fail "bad recursive function binding"
-         end)
-      | _ => fail "recursive values must be functions"
-      end in
-    (x, v)) recs) x.
-Proof.
-  destruct x; reflexivity.
-Qed.
-
-Definition int_to_nat (i : int) : nat :=
-  Z.to_nat (Int63.to_Z i).
-
-Definition int_of_nat n := Uint63.of_Z (Coq.ZArith.BinInt.Z.of_nat n).
-
-#[bypass_check(guard)]
-Fixpoint to_sexp_value (a : value) : sexp :=
-  match a with
-  | Block (i, a) => @Serialize_product _ _ _ (@Serialize_list _ to_sexp_value) (i, List.map (fun j => a.[int_of_nat j]) (seq 0 (int_to_nat (PArray.length a))))
-  | Vec x => Atom "TODO VEC"
-  | Func x => Atom "FUNC"
-  | value_Int x => Atom "TODO INT"
-  | Float x => Atom "TODO FLOAT"
-  | Thunk x => Atom "THUNK"
-  | fail x => Atom ("fail" ++ x)
-  end.
-
-Instance Serialize_value : Serialize value := to_sexp_value.
-
-#[bypass_check(guard)]
 Fixpoint interpret
          (locals : @Ident.Map.t value)
+         (env : @Ident.Map.t value)
          (x : t) {struct x} : value :=
   match x with
   | Mvar v => Ident.Map.find v locals
@@ -213,28 +123,12 @@ Fixpoint interpret
      | [x] => (x, e)
      | x :: xs => (x, Mlambda (xs, e))
     end in
-    Func (fun v => interpret (Ident.Map.add x v locals) e)
-  | Mapply (f_, vs) =>
-     List.fold_left (fun f v => match f with
-     | Func f => f (interpret locals v)
-     | v_wrong => fail ("not a function: " ++ to_string f_ ++ " evaluated to: " ++ to_string v_wrong) end) vs (interpret locals f_)
-  | Mlet (bindings, body) =>
-     let bind :=
-        fix bind (locals : @Ident.Map.t value) (bindings : list binding) : value :=
-        match bindings with
-        | [] => interpret locals body
-        | Unnamed e :: bindings => 
-           let _ := interpret locals e in bind locals bindings
-        | Named (x, e) :: bindings =>
-           let locals := Ident.Map.add x (interpret locals e) (locals) in
-           bind locals bindings
-        | Recursive recs :: bindings =>
-           let newlocals := newlocals interpret recs locals
-            in
-             bind newlocals bindings 
-        end
-     in
-      bind locals bindings 
+    Func (x, locals, e)
+  | Mapply (f, vs) =>
+      match interpret locals env f, vs with
+      | Func (x, locs, e), v :: vs => interpret (Ident.Map.add x (interpret locals env v) locs) env (Mapply (e, vs))
+      | _, _ => fail "not a function"
+      end
   | Mnum (numconst_Int n) => value_Int (Int, Int63.to_Z n)
   (* | Mnum (`Int32 n) -> Int (`Int32, Z.of_int32 n) *)
   (* | Mnum (`Int64 n) -> Int (`Int64, Z.of_int64 n) *)
@@ -245,10 +139,10 @@ Fixpoint interpret
      Vec (Bytevec,
            Array_init (Int63.of_Z (Z.of_nat (String.length s))) (fun i => value_Int (Int, (Z.of_nat (Ascii.nat_of_ascii (option_def Ascii.Space (String.get (Z.to_nat (Int63.to_Z i)) s)))))))
 
-  | Mglobal v => Ident.Map.find v locals
+  | Mglobal _v => fail "globals unsupported"
 
   | Mswitch (scr, cases) =>
-      let scr := interpret locals scr in
+      let scr := interpret locals env scr in
       let fix find_match x := match x with
         | (cases, e) :: rest =>
             if List.existsb (fun case => match case, scr with
@@ -256,19 +150,19 @@ Fixpoint interpret
             | Deftag, Block _ => true
             | Intrange (min, max), value_Int (Int, n) => Z.leb (Int63.to_Z min) n && Z.leb n (Int63.to_Z max)
             | _, _ => false end) cases then
-              interpret locals e
+              interpret locals env e
             else
               find_match rest
         | [] => fail "no case matches" end in
       find_match cases
 
   | Mnumop1 (op, embed_inttype ty, e) =>
-      let n := as_ty ty (interpret locals e) in
+      let n := as_ty ty (interpret locals env e) in
       truncate ty (match op with Neg => Z.mul (-1) n | Not => Z.lnot n end)
 
   | Mnumop2 (op, embed_inttype ty, e1, e2) =>
-      let e1 := interpret locals e1 in
-      let e2 := interpret locals e2 in
+      let e1 := interpret locals env e1 in
+      let e2 := interpret locals env e2 in
       match op with
       | embed_binary_arith_op op =>
           let f := match op with
@@ -305,13 +199,13 @@ Fixpoint interpret
           value_Int (Int, if res then 1%Z else 0%Z)
       end
   | Mnumop1 (Neg, Float64, e) =>
-      Float (- as_float (interpret locals e))
+      Float (- as_float (interpret locals env e))
   | Mnumop1 (Not, Float64, _) 
   | Mnumop2 (embed_binary_bitwise_op _, Float64, _, _) =>
       fail "invalid bitwise float operation"
   | Mnumop2 (embed_binary_arith_op op, Float64, e1, e2) =>
-      let e1 := as_float (interpret locals e1) in
-      let e2 := as_float (interpret locals e2) in
+      let e1 := as_float (interpret locals env e1) in
+      let e2 := as_float (interpret locals env e2) in
       Float (match op with
              | Add => e1 + e2
              | Sub => e1 - e2
@@ -319,8 +213,8 @@ Fixpoint interpret
              | Div => e1 / e2
              | Mod => fail_float "mod on floats not supported" end)
   | Mnumop2 (embed_binary_comparison op, Float64, e1, e2) =>
-      let e1 := as_float (interpret locals e1) in
-      let e2 := as_float (interpret locals e2) in
+      let e1 := as_float (interpret locals env e1) in
+      let e2 := as_float (interpret locals env e2) in
       let res := match op with
              | Lt => PrimFloat.ltb e1 e2
              | Gt => PrimFloat.ltb e2 e2
@@ -331,13 +225,13 @@ Fixpoint interpret
       value_Int (Int, if res then 1%Z else 0%Z)
 
   | Mconvert (embed_inttype src, embed_inttype dst, e) =>
-      truncate dst (as_ty src (interpret locals e))
+      truncate dst (as_ty src (interpret locals env e))
   | Mconvert (embed_inttype src, Float64, e) =>
-      Float (PrimFloat.of_uint63 (Int63.of_Z (as_ty src (interpret locals e))))
+      Float (PrimFloat.of_uint63 (Int63.of_Z (as_ty src (interpret locals env e))))
   | Mconvert (Float64, Float64, e) =>
-      Float (as_float (interpret locals e))
+      Float (as_float (interpret locals env e))
   | Mvecnew (ty, len, def) =>
-      match ty, interpret locals len, interpret locals def with
+      match ty, interpret locals env len, interpret locals env def with
       | Array, value_Int (Int, len), v =>
           Vec (Array, PArray.make (Int63.of_Z len) v)
       | Bytevec, value_Int (Int, len), (value_Int (Int, k)) as v =>
@@ -348,7 +242,7 @@ Fixpoint interpret
       | _, _, _ => fail "bad vector creation"
       end
   | Mvecget (ty, vec, idx) =>
-      (match interpret locals vec, interpret locals idx with
+      (match interpret locals env vec, interpret locals env idx with
        | Vec (ty', vals), value_Int (Int,i) =>
            if vector_type_eqb ty ty' then
              if Z.leb 0 i && Z.ltb i (Int63.to_Z (PArray.length vals)) then
@@ -361,9 +255,9 @@ Fixpoint interpret
        end
       )
   | Mvecset (ty, vec, idx, e) => fail "not implemented"
-      (* (match interpret locals vec, *)
-      (*        interpret locals idx, *)
-      (*        interpret locals e with *)
+      (* (match interpret locals env vec, *)
+      (*        interpret locals env idx, *)
+      (*        interpret locals env e with *)
       (*  | Vec (ty', vals), value_Int (Int, i), v => *)
       (*      if vector_type_eqb ty ty' then *)
       (*        let i := Int63.to_Z i in *)
@@ -373,39 +267,23 @@ Fixpoint interpret
       (*          | Bytevec, Int (Int, i) *)
   (*      else fail "wrong vector type" *)
   | Mveclen (ty, vec) =>
-      match interpret locals vec with
+      match interpret locals env vec with
       | Vec (ty', vals) =>
           if vector_type_eqb ty ty' then value_Int (Int, Int63.to_Z (PArray.length vals)) else fail "wrong vector type"
       | _ => fail "wrong vector type"
       end
   | Mblock (tag, vals) =>
-      Block (tag, Array_of_list (fail "") (List.map (interpret locals) vals))
+      Block (tag, Array_of_list (fail "empty array") (List.map (interpret locals env) vals))
   | Mfield (idx, b) =>
-      match interpret locals b with
+      match interpret locals env b with
       | Block (_, vals) => PArray.get vals idx
       | _ => fail "not a block"
       end
-  | Mlazy e => Thunk (interpret locals e)
+  | Mlazy e => Thunk (interpret locals env e)
   | Mforce e =>
-      match interpret locals e with
+      match interpret locals env e with
       | Thunk v => v
       | _ => fail "not a lazy value"
       end
   | _ => fail "assert todo"
 end.
-
-Definition cond scr case : bool := 
-  (match case, scr with
-    | Tag n, Block (n', _) => Int63.eqb n n'
-    | Deftag, Block _ => true
-    | Intrange (min, max), value_Int (Int, n) => Z.leb (Int63.to_Z min) n && Z.leb n (Int63.to_Z max)
-    | _, _ => false end).
-
-Definition find_match := fun ilocals scr => fix find_match x := match x with
-| (cases, e) :: rest =>
-    if List.existsb (cond scr)  cases then
-      interpret ilocals e
-    else
-      find_match rest
-| [] => fail "no case matches" end.
-
