theories/InterpreterStrictCorrect.v
@@ -1,0 +1,26 @@
+From Malfunction Require InterpreterStrict.
+From Malfunction Require Import Interpreter Malfunction.
+Require Import ZArith String.
+
+Notation sinterpret := InterpreterStrict.interpret.
+Notation svalue := InterpreterStrict.value.
+
+Definition Array_map {A B} (f : A -> B) (a : PArray.array A) :=
+  Array_of_list (f (PArray.default a))
+                (List.map f (List.map (fun n => PArray.get a (Uint63.of_Z (Z.of_nat n))) (List.seq 0 (Z.to_nat (Uint63.to_Z (PArray.length a)))))).
+
+#[bypass_check(guard)]
+Fixpoint vtrans (s : svalue) : value :=
+  match s with
+  | InterpreterStrict.Block (tag, vals) => Block (tag, Array_map vtrans vals)
+  | InterpreterStrict.Vec (ty, vals) => Vec (ty, Array_map vtrans vals)
+  | InterpreterStrict.Func (x, locals, e) => Func (fun v => interpret (Ident.Map.add x v (fun x => vtrans (locals x))) (fun _ => fail "no globals") e)
+  | InterpreterStrict.value_Int (ty, i) => value_Int (ty, i)
+  | InterpreterStrict.Float f => Float f
+  | InterpreterStrict.Thunk v => Thunk (vtrans v)
+  | InterpreterStrict.fail x => fail x
+  end.
+
+
+Theorem interpreter_correct :
+  interpret
