theories/Mcase.v
@@ -1,0 +1,174 @@
+From Malfunction Require Import Malfunction SemanticsSpec.
+From MetaCoq Require Import MCList.
+Require Import List Lia.
+Export ListNotations.
+From MetaCoq Require Import bytestring BasicAst.
+
+Definition Mapply_ '(e, l) :=
+    match l with [] => e | _ => Mapply (e, l) end.
+
+Definition Mlambda_ '(e, l) :=
+    match e with [] => l | _ => Mlambda (e, l) end.
+
+Definition Mcase : t * list (list Ident.t * t) -> t :=
+ fun '(discr, brs) =>
+   Mswitch (discr, mapi (fun i '(nms, b) => ([Malfunction.Tag (int_of_nat i)], Mapply_ (Mlambda_ (nms, b),
+   mapi (fun i _ => Mfield (int_of_nat i, discr)) (nms)))) brs).
+
+Definition add_multiple (nms : list Ident.t) (args : list value) locals :=
+    fold_right (fun '(nm, arg) locals => Ident.Map.add nm arg locals) locals (map2 pair nms args). 
+
+Definition Func_ nms locals b v :=
+  match nms with
+  | n :: nms => Func (n, locals, Mlambda_ (nms, b))
+  | nil => v
+  end.
+
+Fixpoint Mnapply (l : t) (args : list t) :=
+  match args with
+    [] => l
+  | a :: args => Mnapply (Mapply_ (l, [a])) args
+  end.
+
+Lemma Mnapply_app l args1 args2 :
+  Mnapply l (args1 ++ args2) = Mnapply (Mnapply l args1) args2.
+Proof.
+  induction args1 in l, args2 |- *; cbn.
+  - reflexivity.
+  - now rewrite IHargs1.
+Qed. 
+
+Lemma eval_app_nested_ globals locals args l args' v :
+  eval globals locals (Mnapply l (args' ++ args)) v ->
+  eval globals locals (Mapply_ (Mnapply l args', args)) v.
+Proof.
+  induction args in args' |- *.
+  - cbn. now rewrite app_nil_r.
+  - cbn. intros H. specialize (IHargs (args' ++ [a])). destruct args.
+    + now rewrite Mnapply_app in H.
+    + econstructor. cbn in *.
+      rewrite !Mnapply_app in IHargs.
+      eapply IHargs. rewrite Mnapply_app in H. cbn in H.
+      cbn. eauto.
+Qed.
+
+Lemma add_to_add_multiple nm y nms' values' locals :
+  NoDup (nm :: nms') ->
+  #|nms'| = #|values'| ->
+  Ident.Map.add nm y (add_multiple nms' values' locals) =
+  add_multiple (nms' ++ [nm]) (values' ++ [y]) locals.
+Proof.
+  intros H Hlen. induction nms' in values', H, Hlen, nm, y |- *.
+  - destruct values'; cbn in Hlen; try lia. reflexivity.
+  - destruct values'; cbn in Hlen; try lia.
+    cbn.
+    fold (add_multiple (nms') (values') locals).
+    fold (add_multiple (nms' ++ [nm]) (values' ++ [y]) locals).
+    rewrite <- IHnms'.
+    3: lia. 2:{ inversion H; eauto. }
+Admitted.
+
+Lemma NoDup_app {X} (l1 l2 : list X) :
+  NoDup (l1 ++ l2) ->
+  NoDup l1 /\ NoDup l2.
+Proof.
+  induction l1; inversion 1; subst; split; try econstructor; firstorder.
+  rewrite in_app_iff in *; firstorder subst.
+Qed.
+
+Lemma eval_app_ globals locals args values values' nms' nms b v l :
+  #|args| = #|nms| -> 
+  #|nms'| = #|values'| ->
+
+  NoDup (nms' ++ nms) ->
+  Forall2 (eval globals locals) args values ->
+  eval globals (add_multiple (nms' ++ nms) (values' ++ values) locals) b v ->
+  eval globals locals l (Func_ nms (add_multiple nms' values' locals) b v) ->
+  eval globals locals (Mapply_ (l, args)) v.
+Proof.
+  intros Hlen Hlenv Hdup H Heval Hl.
+  eapply (eval_app_nested_ globals locals args l []). cbn.
+  induction args in H, b, nms, nms', Hlen, Heval, v, values, values', Hl, l, Hdup, Hlenv |- *.
+  - cbn. destruct nms; cbn in *; try lia. eauto.
+  - destruct nms as [ | nm nms]; cbn in Hlen. 1: lia.
+    inversion H. subst. rename H2 into Hx.
+    destruct args.
+    + destruct nms; cbn in Hlen; try lia. inversion H4; subst. clear H4.
+      cbn. econstructor; eauto.
+      rewrite add_to_add_multiple; eauto.
+      eapply NoDup_incl_NoDup; eauto. rewrite app_length; cbn; lia. intros ? ?; rewrite in_app_iff in *; firstorder.
+    + destruct nms as [ | nm' nms]. cbn in *; lia.
+      cbn. eapply IHargs with (nms' := nms' ++ [nm]) (values' := values' ++ [y]).
+      5:{ rewrite <- !app_assoc. cbn. eapply Heval. }
+      1: cbn; eauto. 1:{ rewrite !app_length; cbn; lia. } 1:{ rewrite <- !app_assoc. cbn. eauto. } eauto.
+      econstructor; [ eauto.. | ].
+      cbn. destruct nms; rewrite add_to_add_multiple.
+      * econstructor.
+      * assert (nms' ++ [nm; nm'] = (nms' ++ [nm]) ++ [nm']) as Eq by now rewrite <- !app_assoc.
+        rewrite Eq in Hdup. eapply NoDup_app in Hdup as [Hdup _].
+        eapply NoDup_incl_NoDup; eauto. rewrite !app_length; cbn; lia. intros ? ?; rewrite !in_app_iff in *; firstorder subst.
+      * lia.
+      * econstructor. cbn. lia.
+      * assert (nms' ++ nm :: nm' :: t0 :: nms = (nms' ++ [nm]) ++ (nm' :: t0 :: nms)) as Eq by now rewrite <- !app_assoc.
+        rewrite Eq in Hdup. eapply NoDup_app in Hdup as [Hdup _].
+        eapply NoDup_incl_NoDup; eauto. rewrite !app_length; cbn; lia. intros ? ?; rewrite !in_app_iff in *; firstorder subst.
+      * lia.
+Qed.
+
+Lemma eval_apply_lambda globals locals args nms b values v : 
+  #|args| = #|nms| -> 
+  Forall2 (eval globals locals) args values ->
+  eval globals (add_multiple nms values locals) b v ->
+  eval globals locals (Mapply_ (Mlambda_ (nms, b), args)) v.
+Proof.
+  intros.
+  eapply eval_app_ with (nms' := []) (values' := []); eauto.
+  destruct nms.
+  - cbn. eauto.
+  - cbn. destruct nms.
+    + econstructor.
+    + econstructor. cbn. lia.
+Qed.
+
+Lemma eval_case globals locals discr i args brs nms br v :
+  eval globals locals discr (Block (int_of_nat i, args)) ->
+  nth_error brs i = Some (nms, br) -> 
+  NoDup nms ->
+  #|args| = #|nms| ->
+  eval globals (add_multiple nms args locals) br v ->
+  eval globals locals (Mcase (discr, brs)) v.
+Proof.
+  intros Hdiscr Hnth Hdup Hlen Hbr.
+  eapply eval_switch with (e := Mapply_ (Mlambda_ (nms, br), mapi (fun i _ => Mfield (int_of_nat i, discr)) (nms))).
+  - eauto.
+  - clear - Hnth. unfold mapi at 1. change i with (0 + i). 
+    generalize 0 as n. intros n. induction brs as [ | [nms' br'] brs IH] in i, Hnth , nms, br, n |- *.
+    + destruct i; inversion Hnth.
+    + destruct i; cbn in Hnth.
+      * inversion Hnth as [ ]. subst; clear Hnth. cbn.
+        replace (n + 0) with n by lia.
+        now rewrite Bool.orb_false_r, Int63.eqb_refl.
+      * cbn [mapi mapi_rec]. unfold find_match.
+        destruct existsb eqn:E.
+        -- cbn in E. rewrite Bool.orb_false_r in E.
+           eapply Int63.eqb_correct in E.
+           eapply (f_equal int_to_nat) in E.
+           rewrite !int_to_of_nat in E.
+           lia. all:admit.           
+        -- fold find_match. erewrite <- (IH i _ _ _ (S n)). do 4 f_equal. lia.
+  - eapply eval_apply_lambda. 3: eassumption. 1: now rewrite mapi_length.
+    unfold mapi. change 0 with (#|@nil value|).
+    revert Hdiscr. change args with ([] ++ args) at 1. generalize (@nil value) as args'. 
+    intros args' Hdiscr.
+    induction args in nms, Hlen, Hdup, Hdiscr, args' |- *.
+    + destruct nms; inversion Hlen. cbn. econstructor.
+    + destruct nms; inversion Hlen. cbn. econstructor.
+      2: eapply IHargs with (args' := a :: args').
+      * evar (v' : value).
+        enough (a = v') as E. subst v'. rewrite E. econstructor.
+        eapply Hdiscr. admit. admit.
+        subst v'. rewrite int_to_of_nat. 2: admit.
+        rewrite app_nth2, PeanoNat.Nat.sub_diag; [ reflexivity | lia].
+      * now inversion Hdup.
+      * assumption.
+Admitted.
